coq_session/sta_valid.v
@@ -6,7 +6,6 @@ Set Implicit Arguments.
 Unset Strict Implicit.
 Unset Printing Implicit Defensive.
 
-
 Theorem sta_valid Γ m A : Γ ⊢ m : A -> exists s, Γ ⊢ A : Sort s.
 Proof with eauto using sta_type.
   move=>ty. elim: ty=>{Γ m A}...
@@ -85,6 +84,14 @@ Proof with eauto.
     apply: conv_trans... }
 Qed.
 
+Lemma sta_lam0_invY Γ A C m s :
+  Γ ⊢ Lam0 A m s : C -> exists B, (A :: Γ) ⊢ m : B.
+Proof with eauto.
+  move e:(Lam0 A m s)=>n tyL.
+  elim: tyL A m s e=>//{Γ C n}.
+  move=>Γ A B m s tym _ A0 m0 s0[e1 e2 e3]. subst. exists B...
+Qed.
+
 Lemma sta_lam1_invX Γ A1 A2 B C m s1 s2 t :
   Γ ⊢ Lam1 A1 m s1 : C ->
   C === Pi1 A2 B s2 ->
@@ -106,6 +113,14 @@ Proof with eauto.
       s1 s2 t e eq2 tyB0; subst.
     apply: ihm...
     apply: conv_trans... }
+Qed.
+
+Lemma sta_lam1_invY Γ A C m s :
+  Γ ⊢ Lam1 A m s : C -> exists B, (A :: Γ) ⊢ m : B.
+Proof with eauto.
+  move e:(Lam1 A m s)=>n tyL.
+  elim: tyL A m s e=>//{Γ C n}.
+  move=>Γ A B m s tym _ A0 m0 s0[e1 e2 e3]. subst. exists B...
 Qed.
 
 Lemma sta_lam0_inv Γ m A1 A2 B s1 s2 :
